FastMultiplication/ShorVerification/Implementation/QFT/Spec/Assertions.lean
@@ -1,4 +1,5 @@
 import FastMultiplication.ShorVerification.Implementation.QFT.Defs
+import FastMultiplication.ShorVerification.Implementation.QFT.Spec.Cleanliness
 
 /-!
 # QFT Public Assertion
